dfs total correctness

dfs.thy
@@ -28,6 +28,7 @@ definition dfs where
         \<and> {v. reachable \<acute>G \<acute>root v} = \<acute>discovered \<union> (\<Union>v \<in> set \<acute>stack. {w. reachable \<acute>G v w})
         \<and> (\<forall>v \<in> \<acute>discovered. \<forall>w. dominates \<acute>G v w \<longrightarrow> w \<in> \<acute>discovered \<union> set \<acute>stack)
       \<rbrace>
+  VAR (card ({v. reachable \<acute>G \<acute>root v} - \<acute>discovered) <*MLEX*> (MEASURE length \<acute>stack))
   DO
     \<acute>v :== hd \<acute>stack;;
     \<acute>stack :== tl \<acute>stack;;
@@ -38,7 +39,7 @@ definition dfs where
   OD
 "
 
-lemma dfs_spec1:
+lemma dfs_partial1:
 assumes a1: "wf_digraph G"
 and a2: "reachable G v x"
 shows
@@ -60,7 +61,7 @@ shows
   apply (meson a1 wf_digraph.reachable_adjI wf_digraph.reachable_trans)
   done
 
-lemma dfs_spec: "\<Gamma> \<turnstile> \<lbrace> \<acute>root \<in> verts \<acute>G \<and> fin_digraph \<acute>G \<rbrace> dfs \<lbrace> \<acute>discovered = {v. reachable \<acute>G \<acute>root v} \<rbrace>"
+lemma dfs_partial: "\<Gamma> \<turnstile> \<lbrace> \<acute>root \<in> verts \<acute>G \<and> fin_digraph \<acute>G \<rbrace> dfs \<lbrace> \<acute>discovered = {v. reachable \<acute>G \<acute>root v} \<rbrace>"
   unfolding dfs_def apply (vcg; clarsimp simp add: fin_digraph.axioms(1) wf_digraph.reachable_refl)
   apply (subgoal_tac "set (SOME ws. set ws = {pre_digraph.head G e |e. e \<in> arcs G \<and> tail G e = hd stack})
   = {pre_digraph.head G e |e. e \<in> arcs G \<and> tail G e = hd stack}")
@@ -82,7 +83,7 @@ lemma dfs_spec: "\<Gamma> \<turnstile> \<lbrace> \<acute>root \<in> verts \<acut
       apply (subgoal_tac "(hd stack, x) \<in> rtrancl {(u, v). (u, v) \<in> arcs_ends G \<and> {u, v} \<subseteq> discovered}")
        apply (erule_tac ?a1.0="hd stack" in rtrancl.cases; clarsimp)
       apply (subgoal_tac "wf_digraph G")
-       apply (rule dfs_spec1; blast)
+       apply (rule dfs_partial1; blast)
   using fin_digraph.axioms(1) apply fastforce
      apply (metis insertE list.collapse list.simps(15))
     apply (meson list.set_sel(2))
@@ -91,6 +92,53 @@ lemma dfs_spec: "\<Gamma> \<turnstile> \<lbrace> \<acute>root \<in> verts \<acut
    apply (meson finite_list someI_ex)
   using finite_image_set fin_digraph.finite_arcs finite_subset apply fastforce
   done
+
+lemma dfs_total: "\<Gamma> \<turnstile>\<^sub>t \<lbrace> \<acute>root \<in> verts \<acute>G \<and> fin_digraph \<acute>G \<rbrace> dfs \<lbrace> \<acute>discovered = {v. reachable \<acute>G \<acute>root v} \<rbrace>"
+  unfolding dfs_def apply (vcg; clarsimp simp add: fin_digraph.axioms(1) wf_digraph.reachable_refl)
+  apply (subgoal_tac "set (SOME ws. set ws = {pre_digraph.head G e |e. e \<in> arcs G \<and> tail G e = hd stack})
+    = {pre_digraph.head G e |e. e \<in> arcs G \<and> tail G e = hd stack}")
+   apply clarsimp
+   apply (thin_tac "set (SOME ws. set ws = {pre_digraph.head G e |e. e \<in> arcs G \<and> tail G e = hd stack}) =
+           {pre_digraph.head G e |e. e \<in> arcs G \<and> tail G e = hd stack}")
+   apply (safe; clarsimp?)
+                apply (metis Diff_insert0 card_Diff_insert diff_le_self nat_less_le)
+               apply (subgoal_tac "hd stack \<in> discovered")
+                apply blast
+               apply (subgoal_tac "discovered \<union> (\<Union>v\<in>set stack. Collect (reachable G v)) - insert (hd stack) discovered
+                          \<subseteq> discovered \<union> (\<Union>v\<in>set stack. Collect (reachable G v)) - discovered")
+                apply (subgoal_tac "discovered \<union> (\<Union>v\<in>set stack. Collect (reachable G v)) - insert (hd stack) discovered
+                           = discovered \<union> (\<Union>v\<in>set stack. Collect (reachable G v)) - discovered")
+                 apply (smt (verit, del_insts) Diff_iff UN_insert Un_iff fin_digraph.axioms(1) insertI1 list.collapse list.simps(15) mem_Collect_eq subsetD wf_digraph.reachable_refl)
+                apply (subgoal_tac "finite (discovered \<union> (\<Union>v\<in>set stack. Collect (reachable G v)) - discovered)")
+                 apply (meson psubsetI psubset_card_mono)
+                apply (subgoal_tac "finite (Collect (reachable G root))")
+                 apply (metis finite_Diff)
+                apply (metis fin_digraph_axioms_def fin_digraph_def finite_subset mem_Collect_eq reachable_in_vertsE subsetI)
+               apply fastforce
+              apply (simp add: fin_digraph.axioms(1) wf_digraph.head_in_verts)
+             apply (meson in_mono list.set_sel(2))
+            apply (metis insertE list.collapse list.simps(15) pre_digraph.converse_reachable_cases reachableE)
+           apply (meson fin_digraph_def in_mono list.set_sel(1) wf_digraph.reachable_refl)
+          apply (metis arc_to_ends_def fin_digraph.axioms(1) hd_in_set wf_digraph.adj_reachable_trans wf_digraph.dominatesI)
+         apply (meson list.set_sel(2))
+        apply auto[1]
+       apply (metis insertE list.collapse list.simps(15))
+      apply (meson in_mono list.set_sel(2))
+     apply (subgoal_tac "v = hd stack")
+      apply clarsimp
+      apply (subgoal_tac "(hd stack, x) \<in> rtrancl {(u, v). (u, v) \<in> arcs_ends G \<and> {u, v} \<subseteq> discovered}")
+       apply (erule_tac ?a1.0="hd stack" in rtrancl.cases; clarsimp)
+      apply (subgoal_tac "wf_digraph G")
+       apply (rule dfs_partial1; blast)
+  using fin_digraph.axioms(1) apply fastforce
+     apply (metis insertE list.collapse list.simps(15))
+    apply (meson list.set_sel(2))
+   apply (metis insertE list.collapse list.simps(15))
+  apply (subgoal_tac "finite {pre_digraph.head G e |e. e \<in> arcs G \<and> tail G e = hd stack}")
+   apply (meson finite_list someI_ex)
+  using finite_image_set fin_digraph.finite_arcs finite_subset apply fastforce
+  done
+
 end
 
 end
